Added (ts - dts) bounding invariant and helper lemmas

ironfleet/src/Dafny/Distributed/Protocol/RSL/PerformanceProof/Definitions.i.dfy
@@ -11,28 +11,59 @@ module Definitions_i {
 import opened RslTimestampedDistributedSystem_i
 
 // Generic action step time
-ghost const L:Timestamp
+ghost const {:verify false} L:Timestamp
 
-ghost const Ds := DeliveryTime();
-ghost const D:Timestamp
+ghost const {:verify false} Ds := DeliveryTime();
+ghost const {:verify false} D:Timestamp
+ghost const {:verify false} ProcessPacket:Timestamp
+ghost const {:verify false} MbeNewView:Timestamp
+ghost const {:verify false} MbeP2:Timestamp
+ghost const {:verify false} MbeP2a:Timestamp
+ghost const {:verify false} TruncLog:Timestamp
+ghost const {:verify false} MbeDecide:Timestamp
+ghost const {:verify false} MbeExec:Timestamp
+ghost const {:verify false} CheckViewTimeout:Timestamp
+ghost const {:verify false} CheckQuorumOfViewSuspicion:Timestamp
+ghost const {:verify false} MbeSendHeartbeat:Timestamp
 
  //ghost const Gs := StepTime(RslStep);
  //ghost const As := StepTime(AcceptStep);
  //ghost const G:Timestamp
  //ghost const A:Timestamp
 
-function StepToTimeDelta(hstep:RslStep) : Timestamp
+function {:verify false} StepToTimeDelta(hstep:RslStep) : Timestamp
 {
-  L
+  if hstep == RslStep(0) then
+    ProcessPacket
+  else if hstep == RslStep(1) then
+    MbeNewView
+  else if hstep == RslStep(2) then
+    MbeP2
+  else if hstep == RslStep(3) then
+    MbeP2a
+  else if hstep == RslStep(4) then
+    TruncLog
+  else if hstep == RslStep(5) then
+    MbeDecide
+  else if hstep == RslStep(6) then
+    MbeExec
+  else if hstep == RslStep(7) then
+    CheckViewTimeout
+  else if hstep == RslStep(8) then
+    CheckQuorumOfViewSuspicion
+  else if hstep == RslStep(9) then
+    MbeSendHeartbeat
+  else
+    L
 }
 
-function Rsl_NoRecvPerfUpdate(node_pr:Timestamp, hstep:RslStep) : Timestamp
+function {:verify false} Rsl_NoRecvPerfUpdate(node_pr:Timestamp, hstep:RslStep) : Timestamp
 {
   var total_time := TimeAdd2(node_pr, StepToTimeDelta(hstep));
   total_time
 }
 
-function Rsl_RecvPerfUpdate(node_pr:Timestamp, pkt_pr:Timestamp, hstep:RslStep) : Timestamp
+function {:verify false} Rsl_RecvPerfUpdate(node_pr:Timestamp, pkt_pr:Timestamp, hstep:RslStep) : Timestamp
 {
   var deliveryTime := TimeAdd2(pkt_pr, D);
   var handlerStartTime := TimeMax(deliveryTime, node_pr);
@@ -40,30 +71,64 @@ function Rsl_RecvPerfUpdate(node_pr:Timestamp, pkt_pr:Timestamp, hstep:RslStep) 
   total_time
 }
 
-function Rsl_TimeoutPerfUpdate(node_ts:Timestamp, hstep:RslStep) : Timestamp
+function {:verify false} Rsl_TimeoutPerfUpdate(node_ts:Timestamp, hstep:RslStep) : Timestamp
 {
   node_ts + Timeout() + StepToTimeDelta(hstep)
 }
 
-predicate TimeEq(p1:Timestamp, p2:Timestamp)
+predicate {:verify false} TimeEq(p1:Timestamp, p2:Timestamp)
 {
   p1 == p2
 }
 
-predicate TimeLe(p1:Timestamp, p2:Timestamp)
+predicate {:verify false} TimeLe(p1:Timestamp, p2:Timestamp)
 {
   p1 <= p2
 }
 
 
-function TimeBound1aSent() : Timestamp
+function {:verify false} TimeBound1aSent() : Timestamp
 {
-  Timeout() + 2*L
+  Timeout() + ProcessPacket + MbeNewView
 }
 
-function TimeBound1aReceived() : Timestamp
+function {:verify false} TimeBound1aReceived() : Timestamp
 {
   L + D + L
 }
+
+function {:verify false} {:fuel 2} TimeActionRangeInclusive(prevActionIndex:int) : Timestamp
+  requires prevActionIndex >= 0
+{
+  if prevActionIndex == 0 then
+    StepToTimeDelta(RslStep(prevActionIndex))
+  else 
+    TimeActionRangeInclusive(prevActionIndex - 1) + StepToTimeDelta(RslStep(prevActionIndex))
+}
+
+function {:verify false} TimeActionRange(nextActionIndex:int) : Timestamp
+  requires 0 <= nextActionIndex < 10
+{
+  if nextActionIndex == 0 then
+    TimeActionRangeInclusive(9)
+  else
+    TimeActionRangeInclusive(nextActionIndex - 1)
+}
+
+lemma {:verify false} TimeActionRangeHelper_NoRecv(dts:Timestamp, node_ts:Timestamp, nextActionIndex:int)
+  requires 0 < nextActionIndex < 10
+  requires node_ts <= dts + TimeActionRange(nextActionIndex)
+  ensures node_ts + StepToTimeDelta(RslStep(nextActionIndex)) <= dts + TimeActionRange((nextActionIndex+1) % LReplicaNumActions())
+{
+}
+
+lemma TimeActionRangeHelper_Recv(dts:Timestamp, node_ts:Timestamp, dts':Timestamp, node_ts':Timestamp)
+  requires node_ts <= dts + TimeActionRange(0);
+  requires dts' >= node_ts;
+  requires node_ts' == TimeMax(dts', node_ts) + StepToTimeDelta(RslStep(0))
+  ensures node_ts' <= dts' + TimeActionRange(1);
+{
+}
+
 
 }
