ironfleet/src/Dafny/Distributed/Protocol/RSL/PerformanceProof/PerformanceProof.i.dfy
@@ -13,17 +13,21 @@ module RslPerformanceProof_i {
 import opened TimestampedRslPerformanceProof_i
 import opened CommonProof__Constants_i
 
-predicate {:verify false} RslAssumption(s:TimestampedRslState)
+predicate RslAssumption(s:TimestampedRslState)
 {
   |s.t_replicas| > 0
+
+  // TODO: Remove this assumption
+  && (var nextStep := s.t_environment.nextStep; nextStep.LEnvStepHostIos? ==>
+  (forall io :: io in nextStep.ios && io.LIoOpReceive? ==> !io.r.msg.v.RslMessage_Heartbeat?))
 }
 
-predicate {:verify false} RslConsistency(s:TimestampedRslState)
+predicate RslConsistency(s:TimestampedRslState)
 {
   ConstantsAllConsistentInv(UntimestampRslState(s))
 }
 
-predicate {:verify false} ViewAlwaysZero(s:TimestampedRslState)
+predicate ViewAlwaysZero(s:TimestampedRslState)
 {
   && (forall idx:: 0 <= idx < |s.t_replicas|
     ==>
@@ -31,23 +35,34 @@ predicate {:verify false} ViewAlwaysZero(s:TimestampedRslState)
     )
 }
 
-predicate {:verify false} AlwaysInvariant(s:TimestampedRslState)
+predicate AlwaysInvariant(s:TimestampedRslState)
 {
   && ViewAlwaysZero(s)
 }
 
-predicate {:verify false} InitInvariant(s:TimestampedRslState)
+predicate LSchedulerTimeBound(tls:TimestampedLScheduler)
+{
+  0 <= tls.v.nextActionIndex <= 9
+  && TimeLe(tls.ts, tls.dts + TimeActionRange(tls.v.nextActionIndex))
+}
+
+predicate InitInvariant(s:TimestampedRslState)
   requires RslConsistency(s)
 {
   && (0 < |s.t_replicas|
     ==>
     var r := s.t_replicas[0].v.replica.proposer;
-    if s.t_replicas[0].v.nextActionIndex == 0 then
+    (if s.t_replicas[0].v.nextActionIndex == 0 then
       TimeEq(s.t_replicas[0].ts, TimeZero())
     else
       && s.t_replicas[0].v.nextActionIndex == 1
-      && TimeLe(s.t_replicas[0].ts, Timeout() + L)
+      && TimeLe(s.t_replicas[0].ts, Timeout() + ProcessPacket)
     )
+  )
+
+  && (forall idx :: 0 < idx < |s.t_replicas|
+  ==> LSchedulerTimeBound(s.t_replicas[idx])
+  )
 
   && (0 < |s.t_replicas| ==>
   var p := s.t_replicas[0].v.replica.proposer;
@@ -67,7 +82,7 @@ predicate {:verify false} InitInvariant(s:TimestampedRslState)
   )
 }
 
-predicate {:verify false} Phase1aInvariant(s:TimestampedRslState)
+predicate Phase1Invariant(s:TimestampedRslState)
   requires RslConsistency(s)
 {
   && (forall idx :: 0 <= idx < |s.t_replicas|
@@ -91,7 +106,9 @@ predicate {:verify false} Phase1aInvariant(s:TimestampedRslState)
 
   && (forall pkt :: pkt in s.t_environment.sentPackets
       && pkt.msg.v.RslMessage_1a?
-  ==> TimeLe(pkt.msg.ts, TimeBound1aSent())
+      && |s.t_replicas| > 0
+   ==> TimeLe(pkt.msg.ts, TimeBound1aSent())
+      && pkt.msg.v.bal_1a == s.t_replicas[0].v.replica.proposer.max_ballot_i_sent_1a
   )
 
   && (forall idx :: 0 < idx < |s.t_replicas|
@@ -105,7 +122,15 @@ predicate {:verify false} Phase1aInvariant(s:TimestampedRslState)
   )
 }
 
-lemma {:verify false} NextProcessPacket_0_InitGoesToInit(s:TimestampedRslState, s':TimestampedRslState)
+lemma lemma_RslInitImpliesInitInv(s:TimestampedRslState)
+  requires RslAssumption(s);
+  requires TimestampedRslInit(s.constants, s);
+  ensures InitInvariant(s);
+{
+  
+}
+
+lemma lemma_not1_0_InitGoesToInit(s:TimestampedRslState, s':TimestampedRslState)
   requires RslAssumption(s);
   requires ViewAlwaysZero(s)
   requires RslConsistency(s);
@@ -113,7 +138,7 @@ lemma {:verify false} NextProcessPacket_0_InitGoesToInit(s:TimestampedRslState, 
 
   requires s.t_environment.nextStep.LEnvStepHostIos?;
   requires s.t_environment.nextStep.actor == s.constants.config.replica_ids[0];
-  requires s.t_environment.nextStep.nodeStep == RslStep(0);
+  requires s.t_environment.nextStep.nodeStep != RslStep(1);
 
   requires TimestampedRslNextOneReplica(s, s', 0, s.t_environment.nextStep.ios);
 
@@ -122,7 +147,24 @@ lemma {:verify false} NextProcessPacket_0_InitGoesToInit(s:TimestampedRslState, 
 {
 }
 
-lemma {:verify false} NextProcessPacket_j_InitGoesToInit(s:TimestampedRslState, s':TimestampedRslState, j:int)
+lemma lemma_1_0_InitGoesToPhase1(s:TimestampedRslState, s':TimestampedRslState)
+  requires RslAssumption(s);
+  requires ViewAlwaysZero(s)
+  requires RslConsistency(s);
+  requires RslConsistency(s');
+
+  requires s.t_environment.nextStep.LEnvStepHostIos?;
+  requires s.t_environment.nextStep.actor == s.constants.config.replica_ids[0];
+  requires s.t_environment.nextStep.nodeStep == RslStep(1);
+
+  requires TimestampedRslNextOneReplica(s, s', 0, s.t_environment.nextStep.ios);
+
+  requires InitInvariant(s)
+  ensures Phase1Invariant(s')
+{
+}
+
+lemma lemma_a_j_InitGoesToInit(s:TimestampedRslState, s':TimestampedRslState, j:int)
   requires RslAssumption(s);
   requires ViewAlwaysZero(s)
   requires RslConsistency(s);
@@ -141,20 +183,22 @@ lemma {:verify false} NextProcessPacket_j_InitGoesToInit(s:TimestampedRslState, 
 {
 }
 
-lemma MaybeEnterNewView_1_InitGoesToPhase1a(s:TimestampedRslState, s':TimestampedRslState)
+lemma lemma_a_j_Phase1GoesToPhase1(s:TimestampedRslState, s':TimestampedRslState, j:int)
   requires RslAssumption(s);
   requires ViewAlwaysZero(s)
   requires RslConsistency(s);
   requires RslConsistency(s');
+  requires 0 <= j < |s.constants.config.replica_ids|
+
+  requires j > 0;
 
   requires s.t_environment.nextStep.LEnvStepHostIos?;
-  requires s.t_environment.nextStep.actor == s.constants.config.replica_ids[0];
-  requires s.t_environment.nextStep.nodeStep == RslStep(1);
+  requires s.t_environment.nextStep.actor == s.constants.config.replica_ids[j];
 
-  requires TimestampedRslNextOneReplica(s, s', 0, s.t_environment.nextStep.ios);
+  requires TimestampedRslNextOneReplica(s, s', j, s.t_environment.nextStep.ios);
 
-  requires InitInvariant(s)
-  ensures Phase1aInvariant(s')
+  requires Phase1Invariant(s)
+  ensures Phase1Invariant(s')
 {
 }
 
